GenericStability.fst
@@ -16,32 +16,95 @@ open GenericSort
 (**
   filterEq returns the elements of a list that have the same key as n.
 **)
-val filter_eq: #a:Type -> (k:int) -> key:(a -> Tot int) -> (xs: list a) -> Tot (list a)
-let rec filter_eq #a k key xs =
+val filter_eq: #a:Type -> (x:int) -> (xs: list a) -> k:(a -> Tot int) -> Tot (list a)
+let rec filter_eq #a x xs k =
   match xs with
   | [] -> []
   | hd::tl
-    -> if key hd = k then
-        hd::(filter_eq k key tl)
-      else filter_eq k key tl
+    -> if k hd = x then
+        hd::(filter_eq x tl k)
+      else filter_eq x tl k
 
-val filter_eq_contains: #a:eqtype -> (k:int) -> key:(a -> Tot int) -> (xs: list a) ->
-  Lemma(ensures(forall x. (mem x xs /\ key x = k) <==> mem x (filter_eq k key xs)))
-let rec filter_eq_contains #a k key xs =
+val filter_eq_contains: #a:eqtype -> (k:int) -> (xs: list a) -> key:(a -> Tot int) ->
+  Lemma(ensures(forall x. (mem x xs /\ key x = k) <==> mem x (filter_eq k xs key)))
+let rec filter_eq_contains #a k xs key =
   match xs with
   | [] -> ()
   | hd::tl ->
-    if key hd = k then
-      filter_eq_contains k key tl
-    else filter_eq_contains k key tl
+    filter_eq_contains k tl key
 
-val is_stable: x: 'a -> list 'a -> list 'a -> ('a -> Tot int) -> Tot bool
-let is_stable x l1 l2 k = (filter_eq x k l1 = filter_eq x k l2)
+val filter_eq_append: #a:eqtype -> (l1: list a) -> (l2: list a) -> k:(a -> Tot int) ->
+  Lemma(ensures(forall x. (filter_eq x l1 k)@(filter_eq x l2 k) = filter_eq x (l1@l2) k))
+let rec filter_eq_append #a l1 l2 k =
+  match l1 with
+  | [] -> ()
+  | hd::tl ->
+    filter_eq_append tl l2 k
 
-type stable (#a:Type) (l1:list a) (l2:list a) = forall x k. is_stable x l1 l2 k
+val filter_eq_not_contains: #a:eqtype -> (l: list a) -> k:(a -> Tot int) ->
+  Lemma(ensures (forall x. (filter_eq x l k) = [] <==> ~(exists e. (mem e l /\ k e = x))))
+let rec filter_eq_not_contains #a l k =
+  match l with
+  | [] -> ()
+  | hd::tl ->
+    filter_eq_not_contains tl k
 
-(*)
-val filter_eq_ordered: #a:eqtype -> key:(a -> Tot int) -> (xs: list a) ->
-  Lemma(ensures(forall x. ( (Cons.hd xs <> x)  /\ mem x (Cons.tl xs) /\ key (Cons.hd xs) = key x) ==>
-  (Cons.hd xs = Cons.hd (filter_eq (key x) key xs) /\ mem x (Cons.tl (filter_eq (key x) key xs)))))
-let filter_eq_ordered #a (key) xs = ()
+val filter_eq_single: #a:eqtype ->
+  (l: list a{is_Cons l /\ length l = 1}) ->
+  k:(a -> Tot int) ->
+  Lemma(ensures(forall x. (k (hd l) = x ) ==> filter_eq x l k = [hd l]))
+let filter_eq_single #a l k = ()
+
+val filter_eq_sorted_lt:  #a:eqtype -> l:list a{is_Cons l} -> k:(a -> Tot int) ->
+  Lemma(requires (sorted l k))
+  (ensures(forall x. (x < k (hd l)) ==> (filter_eq x l k = [])))
+let filter_eq_sorted_lt #a l k =
+  sorted_lt l k;
+  filter_eq_not_contains l k
+
+val filter_eq_first: #a:eqtype ->
+  (l1: list a{is_Cons l1}) ->
+  (l2: list a{is_Cons l2}) ->
+  k:(a -> Tot int) ->
+  Lemma(requires (sorted l1 k) /\  (k (hd l1) > k (hd l2)))
+  (ensures (forall x. (k (hd l2) = x ) ==>
+    filter_eq x (l1@l2) k = ((filter_eq x ((hd l2)::l1) k )@(filter_eq x (tl l2) k))))
+let filter_eq_first #a l1 l2 k =
+  filter_eq_append l1 l2 k;
+  filter_eq_sorted_lt l1 k
+
+type stable (#a:eqtype) (l1:list a) (l2:list a) (k:(a -> Tot int)) = forall x. (filter_eq x l1 k = filter_eq x l2 k)
+
+val stable_lift: #a:eqtype ->
+  (l1: list a{is_Cons l1}) ->
+  (l2: list a{is_Cons l2}) ->
+  k:(a -> Tot int) ->
+  Lemma(requires (sorted l1 k) /\ (k (hd l1) > k (hd l2)))
+  (ensures (stable (l1@l2) (((hd l2)::l1)@(tl l2)) k))
+let stable_lift #a l1 l2 k =
+  filter_eq_append l1 l2 k;
+  filter_eq_append ((hd l2)::l1) (tl l2) k;
+  filter_eq_first l1 l2 k;
+  filter_eq_append ((hd l2)::l1) (tl l2) k
+
+val stable_append_l: #a:eqtype ->
+  (l: list a) ->
+  (r: list a) ->
+  (r': list a) ->
+  k:(a -> Tot int) ->
+  Lemma(ensures(stable r r' k ==> stable (l@r) (l@r') k))
+let rec stable_append_l #a l r r' k =
+  match l with
+  | [] -> ()
+  | hd::tl -> stable_append_l tl r r' k
+
+val stable_append_r: #a:eqtype ->
+  (l: list a) ->
+  (l': list a) ->
+  (r: list a) ->
+  k:(a -> Tot int) ->
+  Lemma(requires(stable l l' k))
+  (ensures(stable (l@r) (l'@r) k))
+let rec stable_append_r #a l l' r k =
+  filter_eq_append l r k;
+  filter_eq_append l' r k
